Tactics/Sym/AxEffects.lean
@@ -54,7 +54,7 @@ structure AxEffects where
   fields : Std.HashMap StateField AxEffects.FieldEffect
   /-- An expression that contains the proof of:
     ```lean
-    ∀ (f : StateField), f ≠ <f₁> → ⋯ → f ≠ <fₙ> →
+    ∀ (f : StateField), f ∉ [f₁, ⋯, fₙ] →
       r f <currentState> = r f <initialState> `
     ```
     where `f₁, ⋯, fₙ` are the keys of `fields`
@@ -125,9 +125,13 @@ def initial (state : Expr) : AxEffects where
   currentState      := state
   fields            := .empty
   nonEffectProof    :=
-    -- `fun f => rfl`
-    mkLambda `f .default (mkConst ``StateField) <|
-      mkEqReflArmState <| mkApp2 (mkConst ``r) (.bvar 0) state
+    -- `fun (f : StateField) (h : f ∉ []) => rfl`
+    let SF := mkConst ``StateField
+    mkLambda `f .default SF <|
+    let f_nin_nil := -- `f ∉ []`
+      mkNot <| mkStateFieldListMem (.bvar 0) (mkApp (.const ``List.nil [0]) SF)
+    mkLambda `h .default f_nin_nil <|
+      mkEqReflArmState <| mkApp2 (mkConst ``r) (.bvar 1) state
   memoryEffects     := .initial state
   programProof      :=
     -- `rfl`
@@ -192,21 +196,18 @@ private def rewriteType (e eq : Expr) : MetaM Expr := do
 by constructing an application of `eff.nonEffectProof` -/
 partial def mkAppNonEffect (eff : AxEffects) (field : Expr) : MetaM Expr := do
   let msg := m!"constructing application of non-effects proof"
-  withTraceNode msg (tag := "mkAppNonEffect") <| do
-    trace[Tactic.sym] "nonEffectProof: {eff.nonEffectProof}"
+  Sym.withTraceNode msg (tag := "mkAppNonEffect") <| do
+    Sym.traceLargeMsg "nonEffectProof" m!"{eff.nonEffectProof}"
 
     let nonEffectProof := mkApp eff.nonEffectProof field
     let typeOfNonEffects ← inferType nonEffectProof
-    forallTelescope typeOfNonEffects <| fun fvars _ => do
-      trace[Tactic.sym] "hypotheses of nonEffectProof: {fvars}"
-      let lctx ← getLCtx
-      let pre ← fvars.mapM fun expr => do
-        let ty := lctx.get! expr.fvarId! |>.type
-        mkDecideProof ty
+    let (Expr.forallE _name binderType _body _) := typeOfNonEffects
+      | throwError m!"internal error: expected a forall, found:\n  {typeOfNonEffects}"
+    trace[Tactic.sym] "non-effect precondition: {binderType}"
 
-      let nonEffectProof := mkAppN nonEffectProof pre
-      trace[Tactic.sym] "constructed: {nonEffectProof}"
-      return nonEffectProof
+    let nonMemProof ← mkDecideProof binderType
+    Sym.traceLargeMsg "constructed proof of precondition" m!"{nonMemProof}"
+    return mkApp nonEffectProof nonMemProof
 
 /-- Get the value for a field, if one is stored in `eff.fields`,
 or assemble an instantiation of the non-effects proof otherwise -/
@@ -324,8 +325,8 @@ private def update_w (eff : AxEffects) (fld val : Expr) :
   Sym.withTraceNode m!"processing: w {fld} {val} …" (tag := "updateWrite") <| do
   let rField ← reflectStateField fld
 
-  -- Update all other fields
-  let fields ←
+  -- ### Update all other fields
+  let otherFields ←
     eff.fields.toList.filterMapM fun ⟨fld', {value, proof}⟩ => do
       if fld' ≠ rField then
         let proof : Expr ← do
@@ -340,55 +341,80 @@ private def update_w (eff : AxEffects) (fld val : Expr) :
       else
         return none
 
-  -- Update the main field
+  -- ### Update the main field
   let newField : FieldEffect := {
     value := val
     proof :=
       -- `r_of_w_same <fld> <val> <currentState>`
       mkApp3 (mkConst ``r_of_w_same) fld val eff.currentState
   }
-  let fields := (rField, newField) :: fields
+  let fields := (rField, newField) :: otherFields
 
-  -- Update the non-effects proof
-  let nonEffectProof ← lambdaTelescope eff.nonEffectProof fun args proof => do
-    let f := args[0]!
+  -- ### Update the non-effects proof
+  let nonEffectProof ← lambdaBoundedTelescope eff.nonEffectProof 2 fun args proof => do
+    let [f /- : StateField -/, nonMemHyp /- : f ∉ ?modifiedFields -/] := args.toList
+      | throwError "internal error: expected exactly two arguments, found:\
+                    {args}\n\nIn non-effect proof:\n  {eff.nonEffectProof}"
 
-    /- First, assume we have a proof `h_neq : <f> ≠ <fld>`, and use that
-    to compute the new `nonEffectProof` -/
-    let k := fun args h_neq => do
-      let r_of_w := mkApp5 (mkConst ``r_of_w_different)
-                    f fld val eff.currentState h_neq
-      let proof ← mkEqTrans r_of_w proof
-      mkLambdaFVars args proof
-      -- ^^ `fun f ... => Eq.trans (r_of_w_different ... <h_neq>) <proof>`
+    let modifiedFields : Expr /- : List StateField -/ ← do
+      let ty ← inferType nonMemHyp
+      let_expr Not ty := ty
+        | let m ← mkFreshExprMVar none
+          throwError "interal error: expected f ∉ {m}, found:\n  {ty}"
+      let_expr Membership.mem _α _γ _inst _f fields := ty
+        | let m ← mkFreshExprMVar none
+          throwError "interal error: expected f ∈ {m}, found:\n  {ty}"
+      pure fields
 
-    /- Then, determine `h_neq` so that we can pass it to `k`.
-    Notice how we have to modify the environment, to add `h_neq` as a new local
-    hypothesis if it wan't present yet, but only in some branches.
-    This is why we had to define `k` as a monadic continuation,
-    so we can nest `k` under a `withLocalDeclD` -/
-    let h_neq_type := mkApp3 (.const ``Ne [1]) (mkConst ``StateField) f fld
-    let h_neq? ← args.findM? fun h => do
-        let hTy ← inferType h
-        return hTy == h_neq_type
-    match h_neq? with
-      | some h_neq => k args h_neq
-      | none =>
-        let name := Name.mkSimple s!"h_neq_{rField}"
-        withLocalDeclD name h_neq_type fun h_neq =>
-          k (args.push h_neq) h_neq
+    let newProofOfNe := fun oldProof neProof /- : `<f> ≠ <fld>` -/ => do
+      let r_of_w :=
+        mkApp5 (mkConst ``r_of_w_different) f fld val eff.currentState neProof
+      mkEqTrans r_of_w oldProof
 
-  -- Update the memory effects
+    let h? := mkListMemProof 0 (mkConst ``StateField) fld modifiedFields
+    if let some h /- : `<fld> ∈ <modifiedFields>` -/ := h? then
+      -- `fld` was previously modified
+
+      let neProof := -- : `<f> ≠ <fld>`
+        mkNeProofOfMemAndNotMem 0 (mkConst ``StateField) f fld modifiedFields h nonMemHyp
+      -- Adjust the proof
+      let proof ← newProofOfNe proof neProof
+      -- And abstract `f` and `nonMemHyp` again, without changing their types
+      mkLambdaFVars #[f, nonMemHyp] proof
+
+    else
+      -- `fld` was *not* previously modified, so we need to change the type of
+      --   the `nonMemHyp` precondition
+
+      let newModifiedFields := -- `<fld> :: <modifiedFields>`
+        mkApp3 (mkConst ``List.cons) (mkConst ``StateField) fld modifiedFields
+
+      withLocalDeclD `h (mkNot <| mkStateFieldListMem f newModifiedFields) fun newNonMemHyp => do
+        let proof := proof.replaceFVar nonMemHyp <|
+          mkNotMemOfNotMemCons 0 (mkConst ``StateField) f fld
+            modifiedFields newNonMemHyp
+
+        let h := -- : `<fld> ∈ <newModifiedFields>`
+          mkApp3 (.const ``List.Mem.head [0]) (mkConst ``StateField) fld modifiedFields
+        let neProof := -- : `<f> ≠ <fld>`
+          mkNeProofOfMemAndNotMem 0 (mkConst ``StateField) f fld modifiedFields h nonMemHyp
+
+        -- Adjust the proof
+        let proof ← newProofOfNe proof neProof
+        -- And abstract `f` and `newNonMemHyp`
+        mkLambdaFVars #[f, newNonMemHyp] proof
+
+  -- ### Update the memory effects
   let memoryEffects ← eff.memoryEffects.updateWrite eff.currentState fld val
 
-  -- Update the program proof
+  -- ### Update the program proof
   let programProof ←
     -- `Eq.trans (w_program ...) <programProof>`
     mkEqTrans
       (mkAppN (mkConst ``w_program) #[fld, val, eff.currentState])
       eff.programProof
 
-  -- Update the stack alignment proof
+  -- ### Update the stack alignment proof
   let mut sideConditions := eff.sideConditions
   let mut stackAlignmentProof? := eff.stackAlignmentProof?
   if let some proof := stackAlignmentProof? then
